\chapter{Integration}

\begin{equation}
	\int_{-1}^1 \frac{x^2}{1+2^{\sin x}}=\int_{0}^{1} x^2 dx = \frac{1}{3} 1^{3}= \frac{1}{3}
\end{equation}

\begin{thm}
	Let $\even: \real \to \real $ be an even function and $\odd: \real \to \real$ be an odd function. And let $a,b \in \real$. Then
	\begin{equation}
		\int_{-a}^{a} \frac{\even(x)}{1+b^{\odd(x)}} dx = \int_{0}^{a} \even(x) dx
	\end{equation}
\end{thm}

\begin{proof}
  Using that fact that

  \begin{dmath}
    \int_{x=-a}^{x=0} \frac{\even(x)}{1+b^{\odd(x)}} dx
    = \int_{u=a}^{u=0} \frac{\even(-u)}{1+b^{\odd(-u)}} (-1) du
    = \int_{u=0}^{u=a} \left( \frac{\even(u)}{1+b^{-\odd(u)}} \right) \frac{b^{\odd(u)}}{b^{\odd(u)}}du \\
    = \int_{0}^{a} \frac{b^{\odd(u)} \even(u)}{b^\odd(u)+1} du
  \end{dmath}

  We have that
  \begin{dmath}
    \int_{-a}^{a} \frac{\even(x)}{1+b^{\odd(x)}} dx
    = \int_{-a}^{0} \frac{\even(x)}{1+b^{\odd(x)}} dx + \int_{0}^{a} \frac{\even(x)}{1+b^{\odd(x)}} dx
    = \int_{0}^{a} \frac{b^{\odd(x)} \even(x)}{b^{\odd(x)}+1} dx+ \int_{0}^{a} \frac{\even(x)}{1+b^{\odd(x)}} dx
    = \int_{0}^{a} \frac{\even(x) (b^{\odd(x)}+1)}{b^{\odd(x)}+1} dx =
    \int_{0}^{a} \even(x) dx
  \end{dmath}
\end{proof}

\subsection*{100 Integralrechnungen (Weltrekord?)}

\begin{enumerate}
  \item
    \begin{dmath}
      \begin{aligned}
        \int \tan^5 x \sec^3 x dx & = \int \tan^4 x \sec^2 \tan x \sec x dx \\
        &= \int (\tan^2 x)^2 \sec^2 \tan x \sec x dx \\
        &= \int (\sec^2 x-1)^2 \sec^2 \tan x \sec x dx \\
        & \qquad
          \text{Substitution:}
          \quad
          \boxed{\begin{aligned}
              u &:\equiv \sec x\\
              du &:\equiv \sec x \tan x dx
            \end{aligned}
          } \\
        &= \int (u^2-1)^2u^2du \\
        &= \int (u^6-u^4+u^2)du \\
        &= \frac{1}{7} \sec^2x-\frac{2}{5}\sec^5x+\frac{1}{3}\sec^2x+c \\
      \end{aligned}
    \end{dmath}
    \bigbreak
    \hrule
    \bigbreak

  \item
    \begin{dmath}
      \int \frac{ \cos(2x) } {\sin x + \cos x}
      = \int \frac{ \sin^2 x + \cos^2 x } {\sin x + \cos x}
      = \int \frac{ (\cos x - \sin x)(\cos x + \sin x)} {\sin x + \cos x}
      = \int  (\cos x - \sin x) dx
      = \sin x + \cos x + c
    \end{dmath}
    \bigbreak
    \hrule
    \bigbreak

  \item
    \begin{equation}
      \begin{aligned}
        \int\frac{x^2 + 1}{x^4-x^2+1}
        &= \int \frac{1+\frac{1}{x^2}}{x^2-1+\frac{1}{x^2}} \\
        &= \int \frac{1+(1/x^2)}{x^2-2+(1/x^2)+1} \\
        & \qquad
          \text{Substitution:}
          \quad
          \boxed{\begin{aligned}
               u &:\equiv x-\frac{1}{x} \\
              du &:\equiv \left(1+\frac{1}{x^2}\right)dx
                \end{aligned}
          } \\
        &= \int \frac{1}{u^2+1} du \\
        &=\tan^{-1} \left(x-\frac{1}{x}\right)+c
      \end{aligned}
    \end{equation}
    \bigbreak
    \hrule
    \bigbreak

  \item
    \begin{equation}
      \begin{aligned}
        \int (x+e^x)^2 dx
        & = \int (x^2 + 2xe^x+e^{2x}) dx \\
        & \qquad
          \text{DI-method for $2xe^x$:}
          \quad
          \boxed{
            \begin{aligned}
              \begin{array}{ccc}
                & D & I \\
               +& 2x & e^x \\
               -& 2 & e^x \\
               +& 0 & e^x
              \end{array}
            \end{aligned}
          } \\
        & = \frac{1}{3}x^3 + 2xe^x-2e^x+\frac{1}{2}e^{2x}
      \end{aligned}
    \end{equation}
    \bigbreak
    \hrule
    \bigbreak

  \item
    \begin{equation}
      \begin{aligned}
        \int \csc^3 x \sec x \, dx
        & = \int \frac{1}{\sin^3 x \cos x} \, dx \\
        & \qquad
          \text{Pythagorean identity:}
          \quad
          \boxed{
            \begin{aligned}
              \sin^2 \theta + \cos^2 \theta = 1
            \end{aligned}
          } \\
        & = \int \frac{\sin^2 x}{\sin^3 x \cos x} + \frac{\cos^2}{\sin^3 x \cos x} \, dx \\
        & = \int \frac{1}{\sin x \cos x} + \frac{\cos x}{\sin^3 x} \, dx \\
        &  \qquad \text{Pythagorean identity again} \\
        & = \int \frac{\sin^2 x}{\sin x \cos x}+ \frac{\cos^2 x}{\sin x \cos x} + \frac{\cos x}{\sin^3 x} \, dx \\
        & = \int \frac{\sin x}{\cos x} \, dx + \int \frac{\cos x}{\sin x} \, dx + \int \frac{\cos x}{\sin^3 x} \, dx \\
        & = \ln | \sec x | + \ln | \sin x | - \frac{1}{2 \sin^2 x} + c
      \end{aligned}
    \end{equation}
    \bigbreak
    \hrule
    \bigbreak
  %enditem

  \item
    \begin{equation}
      \begin{aligned}
        \int \frac{\cos x}{\sin^2 x - 5 \sin x - 6} \, dx
        & \qquad
        \text{Substitution:}
        \quad
        \boxed{\begin{aligned}
            u &:\equiv \sin x \\
            du &: \equiv \cos x \, dx
          \end{aligned}
        } \\
        & = \int \frac{1}{u^2-5u-6} \, du \\
        & = \int \frac{1/7}{u-6}+\frac{-1/7}{u+1} \, du \\
        & = \frac{1}{7} \ln |u-6| - \frac{1}{7} \ln |u+1| \\
        & = \frac{1}{7} \ln \left | \frac{ \sin x - 6} {\sin x + 1} \right | + c
      \end{aligned}
    \end{equation}

    We have been using the fact that $\frac{1}{u^2-5u-6}=\frac{1}{(u-6)(u+1)}=\frac{a_1}{u-6}+\frac{a_2}{u+1}$ $\iff$ $1=a_1 (u+1) + a_2(u-6)=u(a_1+a_2)+(a_1-6a_2)$. Comparing the coefficients leads to the following system of equations:
    \begin{equation}
      \begin{aligned}
        a_1 & +   a_2 & = 0 \\
        a_1 & - 6 a_2 & = 1
      \end{aligned}
    \end{equation}
    Which implies that $a_1 = \frac{1}{7}$ and $a_2 = -\frac{1}{7}$ and therefore $\frac{1}{u^2-5u-6}=\frac{1}{(u-6)(u+1)}=\frac{1/7}{u-6}+\frac{-1/7}{u+1}$
    \bigbreak
    \hrule
    \bigbreak
  %ENDITEM

  \item
    \begin{equation}
      \int \frac{1}{\sqrt{e^x}} \,dx
       = \int \frac{1}{e^{\frac{x}{2}}} \, dx
       = \int e^{-\frac{x}{2}} \, dx
       = -2 e^{-\frac{x}{2}} = \frac{-2}{\sqrt{e^x}}+c
    \end{equation}

\end{enumerate}